<h2><a href="https://leetcode.com/problems/fibonacci-number/">509. Fibonacci Number</a></h2><h3>Easy</h3><hr><div data-immersive-translate-walked="e006f6e8-8272-4ba2-8087-d07319ea62b3"><p data-immersive-translate-walked="e006f6e8-8272-4ba2-8087-d07319ea62b3" data-immersive-translate-paragraph="1">The <b data-immersive-translate-walked="e006f6e8-8272-4ba2-8087-d07319ea62b3">Fibonacci numbers</b>, commonly denoted <code data-immersive-translate-walked="e006f6e8-8272-4ba2-8087-d07319ea62b3">F(n)</code> form a sequence, called the <b data-immersive-translate-walked="e006f6e8-8272-4ba2-8087-d07319ea62b3">Fibonacci sequence</b>, such that each number is the sum of the two preceding ones, starting from <code data-immersive-translate-walked="e006f6e8-8272-4ba2-8087-d07319ea62b3">0</code> and <code data-immersive-translate-walked="e006f6e8-8272-4ba2-8087-d07319ea62b3">1</code>. That is,</p>

<pre>F(0) = 0, F(1) = 1
F(n) = F(n - 1) + F(n - 2), for n &gt; 1.
</pre>

<p data-immersive-translate-walked="e006f6e8-8272-4ba2-8087-d07319ea62b3" data-immersive-translate-paragraph="1">Given <code data-immersive-translate-walked="e006f6e8-8272-4ba2-8087-d07319ea62b3">n</code>, calculate <code data-immersive-translate-walked="e006f6e8-8272-4ba2-8087-d07319ea62b3">F(n)</code>.</p>

<p data-immersive-translate-walked="e006f6e8-8272-4ba2-8087-d07319ea62b3">&nbsp;</p>
<p data-immersive-translate-walked="e006f6e8-8272-4ba2-8087-d07319ea62b3"><strong class="example" data-immersive-translate-walked="e006f6e8-8272-4ba2-8087-d07319ea62b3" data-immersive-translate-paragraph="1">Example 1:</strong></p>

<pre><strong>Input:</strong> n = 2
<strong>Output:</strong> 1
<strong>Explanation:</strong> F(2) = F(1) + F(0) = 1 + 0 = 1.
</pre>

<p data-immersive-translate-walked="e006f6e8-8272-4ba2-8087-d07319ea62b3"><strong class="example" data-immersive-translate-walked="e006f6e8-8272-4ba2-8087-d07319ea62b3" data-immersive-translate-paragraph="1">Example 2:</strong></p>

<pre><strong>Input:</strong> n = 3
<strong>Output:</strong> 2
<strong>Explanation:</strong> F(3) = F(2) + F(1) = 1 + 1 = 2.
</pre>

<p data-immersive-translate-walked="e006f6e8-8272-4ba2-8087-d07319ea62b3"><strong class="example" data-immersive-translate-walked="e006f6e8-8272-4ba2-8087-d07319ea62b3" data-immersive-translate-paragraph="1">Example 3:</strong></p>

<pre><strong>Input:</strong> n = 4
<strong>Output:</strong> 3
<strong>Explanation:</strong> F(4) = F(3) + F(2) = 2 + 1 = 3.
</pre>

<p data-immersive-translate-walked="e006f6e8-8272-4ba2-8087-d07319ea62b3">&nbsp;</p>
<p data-immersive-translate-walked="e006f6e8-8272-4ba2-8087-d07319ea62b3"><strong data-immersive-translate-walked="e006f6e8-8272-4ba2-8087-d07319ea62b3" data-immersive-translate-paragraph="1">Constraints:</strong></p>

<ul data-immersive-translate-walked="e006f6e8-8272-4ba2-8087-d07319ea62b3">
	<li data-immersive-translate-walked="e006f6e8-8272-4ba2-8087-d07319ea62b3"><code data-immersive-translate-walked="e006f6e8-8272-4ba2-8087-d07319ea62b3">0 &lt;= n &lt;= 30</code></li>
</ul>
</div>